high2/Zeta.High.Verifier.EAC.fsti
@@ -15,3 +15,17 @@ val lemma_neac_implies_hash_collision
   (epmax: epoch)
   (itsl: neac_before_epoch app n epmax {GB.aems_equal_upto epmax itsl})
   : hash_collision app
+
+let provides_hash_collision
+  (#app #n:_)
+  (itsl: Zeta.High.Interleave.neac_log app n)
+  = let open Zeta.High.Interleave in
+    let i = eac_boundary itsl in
+    match Zeta.Interleave.index itsl i with
+    | Zeta.GenericVerifier.AddB _ _ _ _ -> false
+    | _ -> true
+
+val lemma_neac_implies_hash_collision_simple
+  (#app #n:_)
+  (itsl: Zeta.High.Interleave.neac_log app n {provides_hash_collision itsl})
+  : hash_collision app
